code/rsapss/Hacl.Impl.RSAPSS.Keys.fst
@@ -291,45 +291,6 @@ let rsapss_load_skey #t kc rsapss_load_pkey modBits eBits dBits nb eb db skey =
 
 
 inline_for_extraction noextract
-class rsapss_load_keys (t:limb_t) = {
-  load_pkey: rsapss_load_pkey_st t;
-  load_skey: rsapss_load_skey_st t;
-}
-
-
-let load_pkey_u32 : rsapss_load_pkey_st U32 =
-  rsapss_load_pkey mk_runtime_rsapss_checks_uint32
-let load_skey_u32 : rsapss_load_skey_st U32 =
-  rsapss_load_skey mk_runtime_rsapss_checks_uint32 load_pkey_u32
-
-inline_for_extraction noextract
-val mk_runtime_rsapss_load_keys_uint32: rsapss_load_keys U32
-let mk_runtime_rsapss_load_keys_uint32 = {
-  load_pkey = load_pkey_u32;
-  load_skey = load_skey_u32;
-}
-
-let load_pkey_u64 : rsapss_load_pkey_st U64 =
-  rsapss_load_pkey mk_runtime_rsapss_checks_uint64
-let load_skey_u64 : rsapss_load_skey_st U64 =
-  rsapss_load_skey mk_runtime_rsapss_checks_uint64 load_pkey_u64
-
-inline_for_extraction noextract
-val mk_runtime_rsapss_load_keys_uint64: rsapss_load_keys U64
-let mk_runtime_rsapss_load_keys_uint64 = {
-  load_pkey = load_pkey_u64;
-  load_skey = load_skey_u64;
-}
-
-
-inline_for_extraction noextract
-let mk_runtime_rsapss_load_keys (#t:limb_t) : rsapss_load_keys t =
-  match t with
-  | U32 -> mk_runtime_rsapss_load_keys_uint32
-  | U64 -> mk_runtime_rsapss_load_keys_uint64
-
-
-inline_for_extraction noextract
 let new_rsapss_load_pkey_st (t:limb_t) =
     r:HS.rid
   -> modBits:size_t{0 < v modBits}
@@ -356,8 +317,8 @@ let new_rsapss_load_pkey_st (t:limb_t) =
 
 
 inline_for_extraction noextract
-val new_rsapss_load_pkey: #t:limb_t -> kk:rsapss_load_keys t -> new_rsapss_load_pkey_st t
-let new_rsapss_load_pkey #t kk r modBits eBits nb eb =
+val new_rsapss_load_pkey: #t:limb_t -> rsapss_load_pkey:rsapss_load_pkey_st t -> new_rsapss_load_pkey_st t
+let new_rsapss_load_pkey #t rsapss_load_pkey r modBits eBits nb eb =
   [@inline_let] let bits = size (bits t) in
   let nLen = blocks modBits bits in
   let eLen = blocks eBits bits in
@@ -377,7 +338,7 @@ let new_rsapss_load_pkey #t kk r modBits eBits nb eb =
       let pkey: Lib.Buffer.buffer (limb t) = pkey in
       assert (B.length pkey == FStar.UInt32.v pkeyLen);
       let pkey: lbignum t pkeyLen = pkey in
-      let b = kk.load_pkey modBits eBits nb eb pkey in
+      let b = rsapss_load_pkey modBits eBits nb eb pkey in
       let h2 = ST.get () in
       B.(modifies_only_not_unused_in loc_none h0 h2);
       LS.rsapss_load_pkey_lemma #t (v modBits) (v eBits) (as_seq h0 nb) (as_seq h0 eb);
@@ -414,8 +375,8 @@ let new_rsapss_load_skey_st (t:limb_t) =
 
 
 inline_for_extraction noextract
-val new_rsapss_load_skey: #t:limb_t -> kk:rsapss_load_keys t -> new_rsapss_load_skey_st t
-let new_rsapss_load_skey #t kk r modBits eBits dBits nb eb db =
+val new_rsapss_load_skey: #t:limb_t -> rsapss_load_skey:rsapss_load_skey_st t -> new_rsapss_load_skey_st t
+let new_rsapss_load_skey #t rsapss_load_skey r modBits eBits dBits nb eb db =
   [@inline_let] let bits = size (bits t) in
   let nLen = blocks modBits bits in
   let eLen = blocks eBits bits in
@@ -437,7 +398,7 @@ let new_rsapss_load_skey #t kk r modBits eBits dBits nb eb db =
       let skey: Lib.Buffer.buffer (limb t) = skey in
       assert (B.length skey == FStar.UInt32.v skeyLen);
       let skey: lbignum t skeyLen = skey in
-      let b = kk.load_skey modBits eBits dBits nb eb db skey in
+      let b = rsapss_load_skey modBits eBits dBits nb eb db skey in
       let h2 = ST.get () in
       B.(modifies_only_not_unused_in loc_none h0 h2);
       LS.rsapss_load_skey_lemma #t (v modBits) (v eBits) (v dBits)
