code/rsapss/Hacl.RSAPSS.fst
@@ -18,6 +18,17 @@ module BD = Hacl.Bignum.Definitions
 inline_for_extraction noextract
 let t_limbs = U64
 
+private
+[@CInline]
+let load_pkey : RK.rsapss_load_pkey_st t_limbs =
+  RK.rsapss_load_pkey RK.mk_runtime_rsapss_checks
+
+private
+[@CInline]
+let load_skey : RK.rsapss_load_skey_st t_limbs =
+  RK.rsapss_load_skey RK.mk_runtime_rsapss_checks load_pkey
+
+
 val rsapss_sign: len:BN.meta_len t_limbs -> RI.rsapss_sign_st t_limbs (BE.mk_runtime_exp len).BE.mont.BM.bn.BN.len
 let rsapss_sign len a modBits eBits dBits skey sLen salt msgLen msg sgnt =
   RI.rsapss_sign (BE.mk_runtime_exp len) a modBits eBits dBits skey sLen salt msgLen msg sgnt
@@ -27,28 +38,23 @@ val rsapss_verify: len:BN.meta_len t_limbs -> RI.rsapss_verify_st t_limbs (BE.mk
 let rsapss_verify len a modBits eBits pkey sLen k sgnt msgLen msg =
   RI.rsapss_verify (BE.mk_runtime_exp len) a modBits eBits pkey sLen k sgnt msgLen msg
 
-inline_for_extraction noextract
-instance rsapss_inst (len:BN.meta_len t_limbs) : RI.rsapss t_limbs (BE.mk_runtime_exp len) = {
-  RI.rverify = rsapss_verify len;
-  RI.rsign = rsapss_sign len;
-  }
 
 val new_rsapss_load_pkey: RK.new_rsapss_load_pkey_st t_limbs
 let new_rsapss_load_pkey r modBits eBits nb eb =
-  RK.new_rsapss_load_pkey RK.mk_runtime_rsapss_load_keys r modBits eBits nb eb
+  RK.new_rsapss_load_pkey load_pkey r modBits eBits nb eb
 
 
 val new_rsapss_load_skey: RK.new_rsapss_load_skey_st t_limbs
 let new_rsapss_load_skey r modBits eBits dBits nb eb db =
-  RK.new_rsapss_load_skey RK.mk_runtime_rsapss_load_keys r modBits eBits dBits nb eb db
+  RK.new_rsapss_load_skey load_skey r modBits eBits dBits nb eb db
 
 
 val rsapss_skey_sign: len:BN.meta_len t_limbs -> RI.rsapss_skey_sign_st t_limbs (BE.mk_runtime_exp len).BE.mont.BM.bn.BN.len
 let rsapss_skey_sign len a modBits eBits dBits nb eb db sLen salt msgLen msg sgnt =
   RI.rsapss_skey_sign
     (BE.mk_runtime_exp len)
-     RK.mk_runtime_rsapss_load_keys
-    (rsapss_inst len)
+    load_skey
+    (rsapss_sign len)
     a modBits eBits dBits nb eb db sLen salt msgLen msg sgnt
 
 
@@ -56,6 +62,6 @@ val rsapss_pkey_verify: len:BN.meta_len t_limbs -> RI.rsapss_pkey_verify_st t_li
 let rsapss_pkey_verify len a modBits eBits nb eb sLen k sgnt msgLen msg =
   RI.rsapss_pkey_verify
     (BE.mk_runtime_exp len)
-     RK.mk_runtime_rsapss_load_keys
-    (rsapss_inst len)
+    load_pkey
+    (rsapss_verify len)
      a modBits eBits nb eb sLen k sgnt msgLen msg
